src/HOL/Bali/AxCompl.thy
@@ -467,24 +467,6 @@ apply     (erule (3) error_free_field_access)
 apply       (auto dest: eval_type_sound)
 done
 
-(* FIXME To TypeSafe *)
-lemma wf_eval_Fin: 
-  assumes wf:    "wf_prog G" and
-          wt_c1: "\<lparr>prg = G, cls = C, lcl = L\<rparr>\<turnstile>In1r c1\<Colon>Inl (PrimT Void)" and
-        conf_s0: "Norm s0\<Colon>\<preceq>(G, L)" and
-        eval_c1: "G\<turnstile>Norm s0 \<midarrow>c1\<rightarrow> (x1,s1)" and
-        eval_c2: "G\<turnstile>Norm s1 \<midarrow>c2\<rightarrow> s2" and
-            s3: "s3=abupd (abrupt_if (x1\<noteq>None) x1) s2"
-  shows "G\<turnstile>Norm s0 \<midarrow>c1 Finally c2\<rightarrow> s3"
-proof -
-  from eval_c1 wt_c1 wf conf_s0
-  have "error_free (x1,s1)"
-    by (auto dest: eval_type_sound)
-  with eval_c1 eval_c2 s3
-  show ?thesis
-    by - (rule eval.Fin, auto simp add: error_free_def)
-qed
-
 text {* For @{text MGFn_Fin} we need the wellformedness of the program to
 switch from the evaln-semantics to the eval-semantics *}
 lemma MGFn_Fin: 
@@ -559,8 +541,24 @@ apply (rule ax_derivs.Lit [THEN conseq1], tactic "eval_Force_tac 1")
 apply (rule ax_derivs.UnOp, tactic "forw_hyp_eval_Force_tac 1")
 
 apply (rule ax_derivs.BinOp)
-apply  (erule MGFnD [THEN ax_NormalD])
-apply (tactic "forw_hyp_eval_Force_tac 1")
+apply   (erule MGFnD [THEN ax_NormalD])
+
+apply   (rule allI)
+apply   (case_tac "need_second_arg binop v1")
+apply     simp
+apply     (tactic "forw_hyp_eval_Force_tac 1")
+
+apply     simp
+apply     (rule ax_Normal_cases)
+apply       (rule ax_derivs.Skip [THEN conseq1])
+apply       clarsimp
+
+apply       (rule eval_BinOp_arg2_indepI)
+apply       simp
+apply       simp
+
+apply  (rule ax_derivs.Abrupt [THEN conseq1], clarsimp simp add: Let_def)
+apply  (tactic "eval_Force_tac 1")
 
 apply (rule ax_derivs.Super [THEN conseq1], tactic "eval_Force_tac 1")
 apply (erule MGFnD'[THEN conseq12,THEN ax_derivs.Acc],tactic"eval_Force_tac 1")
